Change ModL type

theories/HoareDef.v
@@ -409,7 +409,7 @@ If this feature is needed; we can extend it then. At the moment, I will only all
 
 
   Variable md_tgt: ModL.t.
-  Let ms_tgt: ModSemL.t := (ModL.get_modsem md_tgt (Sk.load_skenv md_tgt.(ModL.sk))).
+  Let ms_tgt: ModSemL.t := (ModL.get_modsem md_tgt md_tgt.(ModL.sk)).
 
   Variable sbtb: list (gname * fspecbody).
   Let stb: list (gname * fspec) := List.map (fun '(gn, fsb) => (gn, fsb_fspec fsb)) sbtb.
@@ -498,20 +498,20 @@ Section SMOD.
   Context `{Σ: GRA.t}.
 
   Record t: Type := mk {
-    get_modsem: SkEnv.t -> SModSem.t;
+    get_modsem: Sk.t -> SModSem.t;
     sk: Sk.t;
   }
   .
 
-  Definition transl (tr: SkEnv.t -> fspecbody -> (Any.t -> itree Es Any.t)) (mr: SModSem.t -> Σ) (md: t): Mod.t := {|
-    Mod.get_modsem := fun skenv => SModSem.transl (tr skenv) mr (md.(get_modsem) skenv);
+  Definition transl (tr: Sk.t -> fspecbody -> (Any.t -> itree Es Any.t)) (mr: SModSem.t -> Σ) (md: t): Mod.t := {|
+    Mod.get_modsem := fun sk => SModSem.transl (tr sk) mr (md.(get_modsem) sk);
     Mod.sk := md.(sk);
   |}
   .
 
   Definition to_src (md: t): Mod.t := transl (fun _ => fun_to_src ∘ fsb_body) (fun _ => ε) md.
   Definition to_mid (md: t): Mod.t := transl (fun _ => fun_to_mid ∘ fsb_body) (fun _ => ε) md.
-  Definition to_tgt (stb: SkEnv.t -> list (gname * fspec)) (md: t): Mod.t := transl (fun_to_tgt ∘ stb) SModSem.initial_mr md.
+  Definition to_tgt (stb: Sk.t -> list (gname * fspec)) (md: t): Mod.t := transl (fun_to_tgt ∘ stb) SModSem.initial_mr md.
 
   (* Definition transl (tr: SModSem.t -> ModSem.t) (md: t): Mod.t := {| *)
   (*   Mod.get_modsem := (SModSem.transl tr) ∘ md.(get_modsem); *)
@@ -522,14 +522,14 @@ Section SMOD.
   (* Definition to_src (md: t): Mod.t := transl SModSem.to_src md. *)
   (* Definition to_mid (md: t): Mod.t := transl SModSem.to_mid md. *)
   (* Definition to_tgt (stb: list (gname * fspec)) (md: t): Mod.t := transl (SModSem.to_tgt stb) md. *)
-  Lemma to_src_comm: forall skenv smd,
-      (SModSem.to_src) (get_modsem smd skenv) = (to_src smd).(Mod.get_modsem) skenv.
+  Lemma to_src_comm: forall sk smd,
+      (SModSem.to_src) (get_modsem smd sk) = (to_src smd).(Mod.get_modsem) sk.
   Proof. refl. Qed.
-  Lemma to_mid_comm: forall skenv smd,
-      (SModSem.to_mid) (get_modsem smd skenv) = (to_mid smd).(Mod.get_modsem) skenv.
+  Lemma to_mid_comm: forall sk smd,
+      (SModSem.to_mid) (get_modsem smd sk) = (to_mid smd).(Mod.get_modsem) sk.
   Proof. refl. Qed.
-  Lemma to_tgt_comm: forall skenv stb smd,
-      (SModSem.to_tgt (stb skenv)) (get_modsem smd skenv) = (to_tgt stb smd).(Mod.get_modsem) skenv.
+  Lemma to_tgt_comm: forall sk stb smd,
+      (SModSem.to_tgt (stb sk)) (get_modsem smd sk) = (to_tgt stb smd).(Mod.get_modsem) sk.
   Proof. refl. Qed.
 
 
@@ -600,9 +600,9 @@ Section SMOD.
   .
   Proof. rewrite ! transl_sk. ss. Qed.
 
-  Definition load_fnsems (skenv: SkEnv.t) (mds: list t) (tr0: fspecbody -> Any.t -> itree Es Any.t) :=
+  Definition load_fnsems (sk: Sk.t) (mds: list t) (tr0: fspecbody -> Any.t -> itree Es Any.t) :=
     do md <- mds;
-    let ms := (get_modsem md skenv) in
+    let ms := (get_modsem md sk) in
       (do '(fn, fsb) <- ms.(SModSem.fnsems);
        let fsem := tr0 fsb in
        ret (fn, transl_all ms.(SModSem.mn) ∘ fsem))
@@ -610,10 +610,10 @@ Section SMOD.
 
   Let transl_fnsems_aux
         tr0 mr0 mds
-        (skenv: SkEnv.t)
+        (sk: Sk.t)
     :
-      (ModSemL.fnsems (ModL.get_modsem (Mod.add_list (List.map (transl tr0 mr0) mds)) skenv)) =
-      (load_fnsems skenv mds (tr0 skenv))
+      (ModSemL.fnsems (ModL.get_modsem (Mod.add_list (List.map (transl tr0 mr0) mds)) sk)) =
+      (load_fnsems sk mds (tr0 sk))
   .
   Proof.
     induction mds; ii; ss.
@@ -621,8 +621,8 @@ Section SMOD.
     rewrite ! List.map_map.
 
     rewrite flat_map_concat_map.
-    replace (fun _x: string * fspecbody => let (fn, fsb) := _x in [(fn, transl_all (SModSem.mn (get_modsem a skenv)) ∘ (tr0 skenv fsb))]) with
-        (ret ∘ (fun _x: string * fspecbody => let (fn, fsb) := _x in (fn, transl_all (SModSem.mn (get_modsem a skenv)) ∘ (tr0 skenv fsb))));
+    replace (fun _x: string * fspecbody => let (fn, fsb) := _x in [(fn, transl_all (SModSem.mn (get_modsem a sk)) ∘ (tr0 sk fsb))]) with
+        (ret ∘ (fun _x: string * fspecbody => let (fn, fsb) := _x in (fn, transl_all (SModSem.mn (get_modsem a sk)) ∘ (tr0 sk fsb))));
       cycle 1.
     { apply func_ext. i. des_ifs. }
     erewrite <- List.map_map with (g:=ret).
@@ -634,7 +634,7 @@ Section SMOD.
         tr0 mr0 mds
     :
       (ModSemL.fnsems (ModL.enclose (Mod.add_list (List.map (transl tr0 mr0) mds)))) =
-      (load_fnsems (Sk.load_skenv (List.fold_right Sk.add Sk.unit (List.map sk mds))) mds (tr0 (Sk.load_skenv (List.fold_right Sk.add Sk.unit (List.map sk mds)))))
+      (load_fnsems (List.fold_right Sk.add Sk.unit (List.map sk mds)) mds (tr0 (List.fold_right Sk.add Sk.unit (List.map sk mds))))
   .
   Proof.
     unfold ModL.enclose.
@@ -674,18 +674,18 @@ Section SMOD.
 
 
 
-  Definition load_initial_mrs (skenv: SkEnv.t) (mds: list t) (mr0: SModSem.t -> Σ): list (string * (Σ * Any.t)) :=
+  Definition load_initial_mrs (sk: Sk.t) (mds: list t) (mr0: SModSem.t -> Σ): list (string * (Σ * Any.t)) :=
     do md <- mds;
-    let ms := (get_modsem md skenv) in
+    let ms := (get_modsem md sk) in
     ret (ms.(SModSem.mn), (mr0 ms, ms.(SModSem.initial_st)))
   .
 
   Let transl_initial_mrs_aux
         tr0 mr0 mds
-        (skenv: SkEnv.t)
+        (sk: Sk.t)
     :
-      (ModSemL.initial_mrs (ModL.get_modsem (Mod.add_list (List.map (transl tr0 mr0) mds)) skenv)) =
-      (load_initial_mrs skenv mds mr0)
+      (ModSemL.initial_mrs (ModL.get_modsem (Mod.add_list (List.map (transl tr0 mr0) mds)) sk)) =
+      (load_initial_mrs sk mds mr0)
   .
   Proof.
     induction mds; ii; ss.
@@ -696,7 +696,7 @@ Section SMOD.
         tr0 mr0 mds
     :
       (ModSemL.initial_mrs (ModL.enclose (Mod.add_list (List.map (transl tr0 mr0) mds)))) =
-      (load_initial_mrs (Sk.load_skenv (List.fold_right Sk.add Sk.unit (List.map sk mds))) mds mr0)
+      (load_initial_mrs (List.fold_right Sk.add Sk.unit (List.map sk mds)) mds mr0)
   .
   Proof.
     unfold ModL.enclose.
