examples/knot/KnotMain01proof.v
@@ -60,8 +60,10 @@ Section SIMMODSEM.
 
   Hypotheses GlobalStb_knot
     :
-      forall skenv,
-        List.find (fun '(_fn, _) => dec "knot" _fn) (GlobalStb skenv) = Some ("knot", knot_spec RecStb FunStb skenv).
+      forall (sk: Sk.t),
+        List.find (fun '(_fn, _) => dec "knot" _fn) (GlobalStb sk) = Some ("knot", knot_spec RecStb FunStb sk).
+
+  Local Opaque Sk.load_skenv.
 
   Theorem correct: ModPair.sim (KnotMain1.Main RecStb GlobalStb) KnotMain0.Main.
   Proof.
